Modify the abstract processor operations to fit Patmos.
This is basically removing most long and float operations,
since Patmos is 32-bit and has no float instructions.
The float instructions will most likely have to be added
in as built-in soft float "instructions" later on.

patmos/Op.v
@@ -41,15 +41,7 @@ Inductive condition : Type :=
   | Ccomp (c: comparison)       (**r signed integer comparison *)
   | Ccompu (c: comparison)      (**r unsigned integer comparison *)
   | Ccompimm (c: comparison) (n: int) (**r signed integer comparison with a constant *)
-  | Ccompuimm (c: comparison) (n: int)  (**r unsigned integer comparison with a constant *)
-  | Ccompl (c: comparison)      (**r signed 64-bit integer comparison *)
-  | Ccomplu (c: comparison)     (**r unsigned 64-bit integer comparison *)
-  | Ccomplimm (c: comparison) (n: int64) (**r signed 64-bit integer comparison with a constant *)
-  | Ccompluimm (c: comparison) (n: int64)  (**r unsigned 64-bit integer comparison with a constant *)
-  | Ccompf (c: comparison)      (**r 64-bit floating-point comparison *)
-  | Cnotcompf (c: comparison)   (**r negation of a floating-point comparison *)
-  | Ccompfs (c: comparison)     (**r 32-bit floating-point comparison *)
-  | Cnotcompfs (c: comparison). (**r negation of a floating-point comparison *)
+  | Ccompuimm (c: comparison) (n: int).  (**r unsigned integer comparison with a constant *)
 
 (** Arithmetic and logical operations.  In the descriptions, [rd] is the
   result of the operation and [r1], [r2], etc, are the arguments. *)
@@ -57,7 +49,6 @@ Inductive condition : Type :=
 Inductive operation : Type :=
   | Omove                    (**r [rd = r1] *)
   | Ointconst (n: int)       (**r [rd] is set to the given integer constant *)
-  | Olongconst (n: int64)    (**r [rd] is set to the given integer constant *)
   | Ofloatconst (n: float)   (**r [rd] is set to the given float constant *)
   | Osingleconst (n: float32)(**r [rd] is set to the given float constant *)
   | Oaddrsymbol (id: ident) (ofs: ptrofs)  (**r [rd] is set to the address of the symbol plus the given offset *)
@@ -72,10 +63,6 @@ Inductive operation : Type :=
   | Omul                     (**r [rd = r1 * r2] *)
   | Omulhs                   (**r [rd = high part of r1 * r2, signed] *)
   | Omulhu                   (**r [rd = high part of r1 * r2, unsigned] *)
-  | Odiv                     (**r [rd = r1 / r2] (signed) *)
-  | Odivu                    (**r [rd = r1 / r2] (unsigned) *)
-  | Omod                     (**r [rd = r1 % r2] (signed) *)
-  | Omodu                    (**r [rd = r1 % r2] (unsigned) *)
   | Oand                     (**r [rd = r1 & r2] *)
   | Oandimm (n: int)         (**r [rd = r1 & n] *)
   | Oor                      (**r [rd = r1 | r2] *)
@@ -89,68 +76,6 @@ Inductive operation : Type :=
   | Oshru                    (**r [rd = r1 >> r2] (unsigned) *)
   | Oshruimm (n: int)        (**r [rd = r1 >> n] (unsigned) *)
   | Oshrximm (n: int)        (**r [rd = r1 / 2^n] (signed) *)
-(*c 64-bit integer arithmetic: *)
-  | Omakelong                (**r [rd = r1 << 32 | r2] *)
-  | Olowlong                 (**r [rd = low-word(r1)] *)
-  | Ohighlong                (**r [rd = high-word(r1)] *)
-  | Ocast32signed            (**r [rd] is 32-bit sign extension of [r1] *)
-  | Ocast32unsigned          (**r [rd] is 32-bit zero extension of [r1] *)
-  | Oaddl                    (**r [rd = r1 + r2] *)
-  | Oaddlimm (n: int64)      (**r [rd = r1 + n] *)
-  | Onegl                    (**r [rd = - r1] *)
-  | Osubl                    (**r [rd = r1 - r2] *)
-  | Omull                    (**r [rd = r1 * r2] *)
-  | Omullhs                  (**r [rd = high part of r1 * r2, signed] *)
-  | Omullhu                  (**r [rd = high part of r1 * r2, unsigned] *)
-  | Odivl                    (**r [rd = r1 / r2] (signed) *)
-  | Odivlu                   (**r [rd = r1 / r2] (unsigned) *)
-  | Omodl                    (**r [rd = r1 % r2] (signed) *)
-  | Omodlu                   (**r [rd = r1 % r2] (unsigned) *)
-  | Oandl                    (**r [rd = r1 & r2] *)
-  | Oandlimm (n: int64)      (**r [rd = r1 & n] *)
-  | Oorl                     (**r [rd = r1 | r2] *)
-  | Oorlimm (n: int64)       (**r [rd = r1 | n] *)
-  | Oxorl                    (**r [rd = r1 ^ r2] *)
-  | Oxorlimm (n: int64)      (**r [rd = r1 ^ n] *)
-  | Oshll                    (**r [rd = r1 << r2] *)
-  | Oshllimm (n: int)        (**r [rd = r1 << n] *)
-  | Oshrl                    (**r [rd = r1 >> r2] (signed) *)
-  | Oshrlimm (n: int)        (**r [rd = r1 >> n] (signed) *)
-  | Oshrlu                   (**r [rd = r1 >> r2] (unsigned) *)
-  | Oshrluimm (n: int)       (**r [rd = r1 >> n] (unsigned) *)
-  | Oshrxlimm (n: int)       (**r [rd = r1 / 2^n] (signed) *)
-(*c Floating-point arithmetic: *)
-  | Onegf                    (**r [rd = - r1] *)
-  | Oabsf                    (**r [rd = abs(r1)] *)
-  | Oaddf                    (**r [rd = r1 + r2] *)
-  | Osubf                    (**r [rd = r1 - r2] *)
-  | Omulf                    (**r [rd = r1 * r2] *)
-  | Odivf                    (**r [rd = r1 / r2] *)
-  | Onegfs                   (**r [rd = - r1] *)
-  | Oabsfs                   (**r [rd = abs(r1)] *)
-  | Oaddfs                   (**r [rd = r1 + r2] *)
-  | Osubfs                   (**r [rd = r1 - r2] *)
-  | Omulfs                   (**r [rd = r1 * r2] *)
-  | Odivfs                   (**r [rd = r1 / r2] *)
-  | Osingleoffloat           (**r [rd] is [r1] truncated to single-precision float *)
-  | Ofloatofsingle           (**r [rd] is [r1] extended to double-precision float *)
-(*c Conversions between int and float: *)
-  | Ointoffloat              (**r [rd = signed_int_of_float64(r1)] *)
-  | Ointuoffloat             (**r [rd = unsigned_int_of_float64(r1)] *)
-  | Ofloatofint              (**r [rd = float64_of_signed_int(r1)] *)
-  | Ofloatofintu             (**r [rd = float64_of_unsigned_int(r1)] *)
-  | Ointofsingle             (**r [rd = signed_int_of_float32(r1)] *)
-  | Ointuofsingle            (**r [rd = unsigned_int_of_float32(r1)] *)
-  | Osingleofint             (**r [rd = float32_of_signed_int(r1)] *)
-  | Osingleofintu            (**r [rd = float32_of_unsigned_int(r1)] *)
-  | Olongoffloat             (**r [rd = signed_long_of_float64(r1)] *)
-  | Olonguoffloat            (**r [rd = unsigned_long_of_float64(r1)] *)
-  | Ofloatoflong             (**r [rd = float64_of_signed_long(r1)] *)
-  | Ofloatoflongu            (**r [rd = float64_of_unsigned_long(r1)] *)
-  | Olongofsingle            (**r [rd = signed_long_of_float32(r1)] *)
-  | Olonguofsingle           (**r [rd = unsigned_long_of_float32(r1)] *)
-  | Osingleoflong            (**r [rd = float32_of_signed_long(r1)] *)
-  | Osingleoflongu           (**r [rd = float32_of_unsigned_int(r1)] *)
 (*c Boolean tests: *)
   | Ocmp (cond: condition).  (**r [rd = 1] if condition holds, [rd = 0] otherwise. *)
 
@@ -159,7 +84,9 @@ Inductive operation : Type :=
 
 Inductive addressing: Type :=
   | Aindexed: ptrofs -> addressing    (**r Address is [r1 + offset] *)
+  | Aindexed2: addressing             (**r Address is [r1 + r2] *)
   | Aglobal: ident -> ptrofs -> addressing  (**r Address is global plus offset *)
+  | Abased: ident -> ptrofs -> addressing (**r Address is [symbol + r1 + offset] *)
   | Ainstack: ptrofs -> addressing.   (**r Address is [stack_pointer + offset] *)
 
 (** Comparison functions (used in modules [CSE] and [Allocation]). *)
@@ -210,14 +137,6 @@ Definition eval_condition (cond: condition) (vl: list val) (m: mem): option bool
   | Ccompu c, v1 :: v2 :: nil => Val.cmpu_bool (Mem.valid_pointer m) c v1 v2
   | Ccompimm c n, v1 :: nil => Val.cmp_bool c v1 (Vint n)
   | Ccompuimm c n, v1 :: nil => Val.cmpu_bool (Mem.valid_pointer m) c v1 (Vint n)
-  | Ccompl c, v1 :: v2 :: nil => Val.cmpl_bool c v1 v2
-  | Ccomplu c, v1 :: v2 :: nil => Val.cmplu_bool (Mem.valid_pointer m) c v1 v2
-  | Ccomplimm c n, v1 :: nil => Val.cmpl_bool c v1 (Vlong n)
-  | Ccompluimm c n, v1 :: nil => Val.cmplu_bool (Mem.valid_pointer m) c v1 (Vlong n)
-  | Ccompf c, v1 :: v2 :: nil => Val.cmpf_bool c v1 v2
-  | Cnotcompf c, v1 :: v2 :: nil => option_map negb (Val.cmpf_bool c v1 v2)
-  | Ccompfs c, v1 :: v2 :: nil => Val.cmpfs_bool c v1 v2
-  | Cnotcompfs c, v1 :: v2 :: nil => option_map negb (Val.cmpfs_bool c v1 v2)
   | _, _ => None
   end.
 
@@ -227,7 +146,6 @@ Definition eval_operation
   match op, vl with
   | Omove, v1::nil => Some v1
   | Ointconst n, nil => Some (Vint n)
-  | Olongconst n, nil => Some (Vlong n)
   | Ofloatconst n, nil => Some (Vfloat n)
   | Osingleconst n, nil => Some (Vsingle n)
   | Oaddrsymbol s ofs, nil => Some (Genv.symbol_address genv s ofs)
@@ -241,10 +159,6 @@ Definition eval_operation
   | Omul, v1 :: v2 :: nil => Some (Val.mul v1 v2)
   | Omulhs, v1::v2::nil => Some (Val.mulhs v1 v2)
   | Omulhu, v1::v2::nil => Some (Val.mulhu v1 v2)
-  | Odiv, v1 :: v2 :: nil => Val.divs v1 v2
-  | Odivu, v1 :: v2 :: nil => Val.divu v1 v2
-  | Omod, v1 :: v2 :: nil => Val.mods v1 v2
-  | Omodu, v1 :: v2 :: nil => Val.modu v1 v2
   | Oand, v1 :: v2 :: nil => Some (Val.and v1 v2)
   | Oandimm n, v1 :: nil => Some (Val.and v1 (Vint n))
   | Oor, v1 :: v2 :: nil => Some (Val.or v1 v2)
@@ -258,65 +172,6 @@ Definition eval_operation
   | Oshru, v1 :: v2 :: nil => Some (Val.shru v1 v2)
   | Oshruimm n, v1 :: nil => Some (Val.shru v1 (Vint n))
   | Oshrximm n, v1::nil => Val.shrx v1 (Vint n)
-  | Omakelong, v1::v2::nil => Some (Val.longofwords v1 v2)
-  | Olowlong, v1::nil => Some (Val.loword v1)
-  | Ohighlong, v1::nil => Some (Val.hiword v1)
-  | Ocast32signed, v1 :: nil => Some (Val.longofint v1)
-  | Ocast32unsigned, v1 :: nil => Some (Val.longofintu v1)
-  | Oaddl, v1 :: v2 :: nil => Some (Val.addl v1 v2)
-  | Oaddlimm n, v1::nil => Some (Val.addl v1 (Vlong n))
-  | Onegl, v1::nil => Some (Val.negl v1)
-  | Osubl, v1::v2::nil => Some (Val.subl v1 v2)
-  | Omull, v1::v2::nil => Some (Val.mull v1 v2)
-  | Omullhs, v1::v2::nil => Some (Val.mullhs v1 v2)
-  | Omullhu, v1::v2::nil => Some (Val.mullhu v1 v2)
-  | Odivl, v1::v2::nil => Val.divls v1 v2
-  | Odivlu, v1::v2::nil => Val.divlu v1 v2
-  | Omodl, v1::v2::nil => Val.modls v1 v2
-  | Omodlu, v1::v2::nil => Val.modlu v1 v2
-  | Oandl, v1::v2::nil => Some(Val.andl v1 v2)
-  | Oandlimm n, v1::nil => Some (Val.andl v1 (Vlong n))
-  | Oorl, v1::v2::nil => Some(Val.orl v1 v2)
-  | Oorlimm n, v1::nil => Some (Val.orl v1 (Vlong n))
-  | Oxorl, v1::v2::nil => Some(Val.xorl v1 v2)
-  | Oxorlimm n, v1::nil => Some (Val.xorl v1 (Vlong n))
-  | Oshll, v1::v2::nil => Some (Val.shll v1 v2)
-  | Oshllimm n, v1::nil => Some (Val.shll v1 (Vint n))
-  | Oshrl, v1::v2::nil => Some (Val.shrl v1 v2)
-  | Oshrlimm n, v1::nil => Some (Val.shrl v1 (Vint n))
-  | Oshrlu, v1::v2::nil => Some (Val.shrlu v1 v2)
-  | Oshrluimm n, v1::nil => Some (Val.shrlu v1 (Vint n))
-  | Oshrxlimm n, v1::nil => Val.shrxl v1 (Vint n)
-  | Onegf, v1::nil => Some (Val.negf v1)
-  | Oabsf, v1::nil => Some (Val.absf v1)
-  | Oaddf, v1::v2::nil => Some (Val.addf v1 v2)
-  | Osubf, v1::v2::nil => Some (Val.subf v1 v2)
-  | Omulf, v1::v2::nil => Some (Val.mulf v1 v2)
-  | Odivf, v1::v2::nil => Some (Val.divf v1 v2)
-  | Onegfs, v1::nil => Some (Val.negfs v1)
-  | Oabsfs, v1::nil => Some (Val.absfs v1)
-  | Oaddfs, v1::v2::nil => Some (Val.addfs v1 v2)
-  | Osubfs, v1::v2::nil => Some (Val.subfs v1 v2)
-  | Omulfs, v1::v2::nil => Some (Val.mulfs v1 v2)
-  | Odivfs, v1::v2::nil => Some (Val.divfs v1 v2)
-  | Osingleoffloat, v1::nil => Some (Val.singleoffloat v1)
-  | Ofloatofsingle, v1::nil => Some (Val.floatofsingle v1)
-  | Ointoffloat, v1::nil => Val.intoffloat v1
-  | Ointuoffloat, v1::nil => Val.intuoffloat v1
-  | Ofloatofint, v1::nil => Val.floatofint v1
-  | Ofloatofintu, v1::nil => Val.floatofintu v1
-  | Ointofsingle, v1::nil => Val.intofsingle v1
-  | Ointuofsingle, v1::nil => Val.intuofsingle v1
-  | Osingleofint, v1::nil => Val.singleofint v1
-  | Osingleofintu, v1::nil => Val.singleofintu v1
-  | Olongoffloat, v1::nil => Val.longoffloat v1
-  | Olonguoffloat, v1::nil => Val.longuoffloat v1
-  | Ofloatoflong, v1::nil => Val.floatoflong v1
-  | Ofloatoflongu, v1::nil => Val.floatoflongu v1
-  | Olongofsingle, v1::nil => Val.longofsingle v1
-  | Olonguofsingle, v1::nil => Val.longuofsingle v1
-  | Osingleoflong, v1::nil => Val.singleoflong v1
-  | Osingleoflongu, v1::nil => Val.singleoflongu v1
   | Ocmp c, _ => Some (Val.of_optbool (eval_condition c vl m))
   | _, _ => None
   end.
@@ -326,7 +181,9 @@ Definition eval_addressing
     (addr: addressing) (vl: list val) : option val :=
   match addr, vl with
   | Aindexed n, v1 :: nil => Some (Val.offset_ptr v1 n)
+  | Aindexed2, v1 :: v2 :: nil => Some (Val.add v1 v2)
   | Aglobal s ofs, nil => Some (Genv.symbol_address genv s ofs)
+  | Abased s ofs, v1 :: nil => Some (Val.add (Genv.symbol_address genv s ofs) v1)
   | Ainstack n, nil => Some (Val.offset_ptr sp n)
   | _, _ => None
   end.
@@ -369,21 +226,12 @@ Definition type_of_condition (c: condition) : list typ :=
   | Ccompu _ => Tint :: Tint :: nil
   | Ccompimm _ _ => Tint :: nil
   | Ccompuimm _ _ => Tint :: nil
-  | Ccompl _ => Tlong :: Tlong :: nil
-  | Ccomplu _ => Tlong :: Tlong :: nil
-  | Ccomplimm _ _ => Tlong :: nil
-  | Ccompluimm _ _ => Tlong :: nil
-  | Ccompf _ => Tfloat :: Tfloat :: nil
-  | Cnotcompf _ => Tfloat :: Tfloat :: nil
-  | Ccompfs _ => Tsingle :: Tsingle :: nil
-  | Cnotcompfs _ => Tsingle :: Tsingle :: nil
   end.
 
 Definition type_of_operation (op: operation) : list typ * typ :=
   match op with
   | Omove => (nil, Tint)   (* treated specially *)
   | Ointconst _ => (nil, Tint)
-  | Olongconst _ => (nil, Tlong)
   | Ofloatconst f => (nil, Tfloat)
   | Osingleconst f => (nil, Tsingle)
   | Oaddrsymbol _ _ => (nil, Tptr)
@@ -397,10 +245,6 @@ Definition type_of_operation (op: operation) : list typ * typ :=
   | Omul => (Tint :: Tint :: nil, Tint)
   | Omulhs => (Tint :: Tint :: nil, Tint)
   | Omulhu => (Tint :: Tint :: nil, Tint)
-  | Odiv => (Tint :: Tint :: nil, Tint)
-  | Odivu => (Tint :: Tint :: nil, Tint)
-  | Omod => (Tint :: Tint :: nil, Tint)
-  | Omodu => (Tint :: Tint :: nil, Tint)
   | Oand => (Tint :: Tint :: nil, Tint)
   | Oandimm _ => (Tint :: nil, Tint)
   | Oor => (Tint :: Tint :: nil, Tint)
@@ -414,72 +258,15 @@ Definition type_of_operation (op: operation) : list typ * typ :=
   | Oshru => (Tint :: Tint :: nil, Tint)
   | Oshruimm _ => (Tint :: nil, Tint)
   | Oshrximm _ => (Tint :: nil, Tint)
-  | Omakelong => (Tint :: Tint :: nil, Tlong)
-  | Olowlong => (Tlong :: nil, Tint)
-  | Ohighlong => (Tlong :: nil, Tint)
-  | Ocast32signed => (Tint :: nil, Tlong)
-  | Ocast32unsigned => (Tint :: nil, Tlong)
-  | Oaddl => (Tlong :: Tlong :: nil, Tlong)
-  | Oaddlimm _ => (Tlong :: nil, Tlong)
-  | Onegl => (Tlong :: nil, Tlong)
-  | Osubl => (Tlong :: Tlong :: nil, Tlong)
-  | Omull => (Tlong :: Tlong :: nil, Tlong)
-  | Omullhs => (Tlong :: Tlong :: nil, Tlong)
-  | Omullhu => (Tlong :: Tlong :: nil, Tlong)
-  | Odivl => (Tlong :: Tlong :: nil, Tlong)
-  | Odivlu => (Tlong :: Tlong :: nil, Tlong)
-  | Omodl => (Tlong :: Tlong :: nil, Tlong)
-  | Omodlu => (Tlong :: Tlong :: nil, Tlong)
-  | Oandl => (Tlong :: Tlong :: nil, Tlong)
-  | Oandlimm _ => (Tlong :: nil, Tlong)
-  | Oorl => (Tlong :: Tlong :: nil, Tlong)
-  | Oorlimm _ => (Tlong :: nil, Tlong)
-  | Oxorl => (Tlong :: Tlong :: nil, Tlong)
-  | Oxorlimm _ => (Tlong :: nil, Tlong)
-  | Oshll => (Tlong :: Tint :: nil, Tlong)
-  | Oshllimm _ => (Tlong :: nil, Tlong)
-  | Oshrl => (Tlong :: Tint :: nil, Tlong)
-  | Oshrlimm _ => (Tlong :: nil, Tlong)
-  | Oshrlu => (Tlong :: Tint :: nil, Tlong)
-  | Oshrluimm _ => (Tlong :: nil, Tlong)
-  | Oshrxlimm _ => (Tlong :: nil, Tlong)
-  | Onegf => (Tfloat :: nil, Tfloat)
-  | Oabsf => (Tfloat :: nil, Tfloat)
-  | Oaddf => (Tfloat :: Tfloat :: nil, Tfloat)
-  | Osubf => (Tfloat :: Tfloat :: nil, Tfloat)
-  | Omulf => (Tfloat :: Tfloat :: nil, Tfloat)
-  | Odivf => (Tfloat :: Tfloat :: nil, Tfloat)
-  | Onegfs => (Tsingle :: nil, Tsingle)
-  | Oabsfs => (Tsingle :: nil, Tsingle)
-  | Oaddfs => (Tsingle :: Tsingle :: nil, Tsingle)
-  | Osubfs => (Tsingle :: Tsingle :: nil, Tsingle)
-  | Omulfs => (Tsingle :: Tsingle :: nil, Tsingle)
-  | Odivfs => (Tsingle :: Tsingle :: nil, Tsingle)
-  | Osingleoffloat => (Tfloat :: nil, Tsingle)
-  | Ofloatofsingle => (Tsingle :: nil, Tfloat)
-  | Ointoffloat => (Tfloat :: nil, Tint)
-  | Ointuoffloat => (Tfloat :: nil, Tint)
-  | Ofloatofint => (Tint :: nil, Tfloat)
-  | Ofloatofintu => (Tint :: nil, Tfloat)
-  | Ointofsingle => (Tsingle :: nil, Tint)
-  | Ointuofsingle => (Tsingle :: nil, Tint)
-  | Osingleofint => (Tint :: nil, Tsingle)
-  | Osingleofintu => (Tint :: nil, Tsingle)
-  | Olongoffloat => (Tfloat :: nil, Tlong)
-  | Olonguoffloat => (Tfloat :: nil, Tlong)
-  | Ofloatoflong => (Tlong :: nil, Tfloat)
-  | Ofloatoflongu => (Tlong :: nil, Tfloat)
-  | Olongofsingle => (Tsingle :: nil, Tlong)
-  | Olonguofsingle => (Tsingle :: nil, Tlong)
-  | Osingleoflong => (Tlong :: nil, Tsingle)
-  | Osingleoflongu => (Tlong :: nil, Tsingle)
   | Ocmp c => (type_of_condition c, Tint)
   end.
 
 Definition type_of_addressing (addr: addressing) : list typ :=
   match addr with
   | Aindexed _ => Tptr :: nil
+  | Aindexed2 => Tptr :: Tptr :: nil
   | Aglobal _ _ => nil
+  | Abased _ _ => Tptr :: nil
   | Ainstack _ => nil
   end.
 
@@ -514,12 +301,11 @@ Proof with (try exact I; try reflexivity; auto using Val.Vptr_has_type).
   destruct op; simpl; simpl in H0; FuncInv; subst; simpl.
   (* move *)
   - congruence.
-  (* intconst, longconst, floatconst, singleconst *)
+  (* intconst, floatconst, singleconst *)
   - exact I.
   - exact I.
   - exact I.
-  - exact I.
-  (* addrsymbol *)
+  (* addrsymbol *) 
   - unfold Genv.symbol_address. destruct (Genv.find_symbol genv id)...
   (* addrstack *)
   - destruct sp... apply Val.Vptr_has_type.
@@ -538,16 +324,6 @@ Proof with (try exact I; try reflexivity; auto using Val.Vptr_has_type).
   - destruct v0; destruct v1...
   - destruct v0; destruct v1...
   - destruct v0; destruct v1...
-  (* div, divu *)
-  - destruct v0; destruct v1; simpl in *; inv H0.
-    destruct (Int.eq i0 Int.zero || Int.eq i (Int.repr Int.min_signed) && Int.eq i0 Int.mone); inv H2...
-  - destruct v0; destruct v1; simpl in *; inv H0.
-    destruct (Int.eq i0 Int.zero); inv H2...
-  (* mod, modu *)
-  - destruct v0; destruct v1; simpl in *; inv H0.
-    destruct (Int.eq i0 Int.zero || Int.eq i (Int.repr Int.min_signed) && Int.eq i0 Int.mone); inv H2...
-  - destruct v0; destruct v1; simpl in *; inv H0.
-    destruct (Int.eq i0 Int.zero); inv H2...
   (* and, andimm *)
   - destruct v0; destruct v1...
   - destruct v0...
@@ -568,100 +344,6 @@ Proof with (try exact I; try reflexivity; auto using Val.Vptr_has_type).
   - destruct v0; simpl... destruct (Int.ltu n Int.iwordsize)...
   (* shrx *)
   - destruct v0; simpl in H0; try discriminate. destruct (Int.ltu n (Int.repr 31)); inv H0...
-  (* makelong, lowlong, highlong *)
-  - destruct v0; destruct v1...
-  - destruct v0...
-  - destruct v0...
-  (* cast32 *)
-  - destruct v0...
-  - destruct v0...
-  (* addl, addlimm *)
-  - apply type_addl.
-  - apply type_addl.
-  (* negl, subl *)
-  - destruct v0...
-  - unfold Val.subl. destruct v0; destruct v1... 
-    unfold Val.has_type; destruct Archi.ptr64...
-    destruct Archi.ptr64... destruct (eq_block b b0)...
-  (* mull, mullhs, mullhu *)
-  - destruct v0; destruct v1...
-  - destruct v0; destruct v1...
-  - destruct v0; destruct v1...
-  (* divl, divlu *)
-  - destruct v0; destruct v1; simpl in *; inv H0.
-    destruct (Int64.eq i0 Int64.zero || Int64.eq i (Int64.repr Int64.min_signed) && Int64.eq i0 Int64.mone); inv H2...
-  - destruct v0; destruct v1; simpl in *; inv H0.
-    destruct (Int64.eq i0 Int64.zero); inv H2...
-  (* modl, modlu *)
-  - destruct v0; destruct v1; simpl in *; inv H0.
-    destruct (Int64.eq i0 Int64.zero || Int64.eq i (Int64.repr Int64.min_signed) && Int64.eq i0 Int64.mone); inv H2...
-  - destruct v0; destruct v1; simpl in *; inv H0.
-    destruct (Int64.eq i0 Int64.zero); inv H2...
-  (* andl, andlimm *)
-  - destruct v0; destruct v1...
-  - destruct v0...
-  (* orl, orlimm *)
-  - destruct v0; destruct v1...
-  - destruct v0...
-  (* xorl, xorlimm *)
-  - destruct v0; destruct v1...
-  - destruct v0...
-  (* shll, shllimm *)
-  - destruct v0; destruct v1; simpl... destruct (Int.ltu i0 Int64.iwordsize')...
-  - destruct v0; simpl... destruct (Int.ltu n Int64.iwordsize')...
-  (* shr, shrimm *)
-  - destruct v0; destruct v1; simpl... destruct (Int.ltu i0 Int64.iwordsize')...
-  - destruct v0; simpl... destruct (Int.ltu n Int64.iwordsize')...
-  (* shru, shruimm *)
-  - destruct v0; destruct v1; simpl... destruct (Int.ltu i0 Int64.iwordsize')...
-  - destruct v0; simpl... destruct (Int.ltu n Int64.iwordsize')...
-  (* shrxl *)
-  - destruct v0; simpl in H0; try discriminate. destruct (Int.ltu n (Int.repr 63)); inv H0...
-  (* negf, absf *)
-  - destruct v0...
-  - destruct v0...
-  (* addf, subf *)
-  - destruct v0; destruct v1...
-  - destruct v0; destruct v1...
-  (* mulf, divf *)
-  - destruct v0; destruct v1...
-  - destruct v0; destruct v1...
-  (* negfs, absfs *)
-  - destruct v0...
-  - destruct v0...
-  (* addfs, subfs *)
-  - destruct v0; destruct v1...
-  - destruct v0; destruct v1...
-  (* mulfs, divfs *)
-  - destruct v0; destruct v1...
-  - destruct v0; destruct v1...
-  (* singleoffloat, floatofsingle *)
-  - destruct v0...
-  - destruct v0...
-  (* intoffloat, intuoffloat *)
-  - destruct v0; simpl in H0; inv H0. destruct (Float.to_int f); inv H2...
-  - destruct v0; simpl in H0; inv H0. destruct (Float.to_intu f); inv H2...
-  (* floatofint, floatofintu *)
-  - destruct v0; simpl in H0; inv H0...
-  - destruct v0; simpl in H0; inv H0...
-  (* intofsingle, intuofsingle *)
-  - destruct v0; simpl in H0; inv H0. destruct (Float32.to_int f); inv H2...
-  - destruct v0; simpl in H0; inv H0. destruct (Float32.to_intu f); inv H2...
-  (* singleofint, singleofintu *)
-  - destruct v0; simpl in H0; inv H0...
-  - destruct v0; simpl in H0; inv H0...
-  (* longoffloat, longuoffloat *)
-  - destruct v0; simpl in H0; inv H0. destruct (Float.to_long f); inv H2...
-  - destruct v0; simpl in H0; inv H0. destruct (Float.to_longu f); inv H2...
-  (* floatoflong, floatoflongu *)
-  - destruct v0; simpl in H0; inv H0...
-  - destruct v0; simpl in H0; inv H0...
-  (* longofsingle, longuofsingle *)
-  - destruct v0; simpl in H0; inv H0. destruct (Float32.to_long f); inv H2...
-  - destruct v0; simpl in H0; inv H0. destruct (Float32.to_longu f); inv H2...
-  (* singleoflong, singleoflongu *)
-  - destruct v0; simpl in H0; inv H0...
-  - destruct v0; simpl in H0; inv H0...
   (* cmp *)
   - destruct (eval_condition cond vl m)... destruct b...
 Qed.
@@ -700,14 +382,6 @@ Definition negate_condition (cond: condition): condition :=
   | Ccompu c => Ccompu(negate_comparison c)
   | Ccompimm c n => Ccompimm (negate_comparison c) n
   | Ccompuimm c n => Ccompuimm (negate_comparison c) n
-  | Ccompl c => Ccompl(negate_comparison c)
-  | Ccomplu c => Ccomplu(negate_comparison c)
-  | Ccomplimm c n => Ccomplimm (negate_comparison c) n
-  | Ccompluimm c n => Ccompluimm (negate_comparison c) n
-  | Ccompf c => Cnotcompf c
-  | Cnotcompf c => Ccompf c
-  | Ccompfs c => Cnotcompfs c
-  | Cnotcompfs c => Ccompfs c
   end.
 
 Lemma eval_negate_condition:
@@ -719,14 +393,6 @@ Proof.
   repeat (destruct vl; auto). apply Val.negate_cmpu_bool.
   repeat (destruct vl; auto). apply Val.negate_cmp_bool.
   repeat (destruct vl; auto). apply Val.negate_cmpu_bool.
-  repeat (destruct vl; auto). apply Val.negate_cmpl_bool.
-  repeat (destruct vl; auto). apply Val.negate_cmplu_bool.
-  repeat (destruct vl; auto). apply Val.negate_cmpl_bool.
-  repeat (destruct vl; auto). apply Val.negate_cmplu_bool.
-  repeat (destruct vl; auto).
-  repeat (destruct vl; auto). destruct (Val.cmpf_bool c v v0) as [[]|]; auto.
-  repeat (destruct vl; auto).
-  repeat (destruct vl; auto). destruct (Val.cmpfs_bool c v v0) as [[]|]; auto.
 Qed.
 
 (** Shifting stack-relative references.  This is used in [Stacking]. *)
@@ -780,7 +446,9 @@ Qed.
 Definition offset_addressing (addr: addressing) (delta: Z) : option addressing :=
   match addr with
   | Aindexed n => Some(Aindexed (Ptrofs.add n (Ptrofs.repr delta)))
+  | Aindexed2 => None
   | Aglobal id n => Some(Aglobal id (Ptrofs.add n (Ptrofs.repr delta)))
+  | Abased id n => Some(Abased id (Ptrofs.add n (Ptrofs.repr delta)))
   | Ainstack n => Some(Ainstack (Ptrofs.add n (Ptrofs.repr delta)))
   end.
 
@@ -801,7 +469,12 @@ Proof.
 - rewrite A; auto.
 - unfold Genv.symbol_address. destruct (Genv.find_symbol ge i); auto. 
   simpl. rewrite H1. f_equal; f_equal; f_equal. symmetry; auto with ptrofs.
-- rewrite A; auto.
+- unfold Genv.symbol_address. destruct (Genv.find_symbol ge i); auto.
+  rewrite Val.add_assoc. rewrite Val.add_permut. rewrite Val.add_commut.
+  simpl; rewrite H1.
+  assert (D: Ptrofs.repr delta = Ptrofs.of_int (Int.repr delta)) by (symmetry; auto with ptrofs).
+  rewrite D. auto.
+- rewrite A. auto.
 Qed.
 
 (** Operations that are so cheap to recompute that CSE should not factor them out. *)
@@ -809,8 +482,8 @@ Qed.
 Definition is_trivial_op (op: operation) : bool :=
   match op with
   | Omove => true
-  | Ointconst n => Int.eq (Int.sign_ext 12 n) n
-  | Olongconst n => Int64.eq (Int64.sign_ext 12 n) n
+  | Ointconst _ => true
+  | Oaddrsymbol _ _ => true
   | Oaddrstack _ => true
   | _ => false
   end.
@@ -821,8 +494,6 @@ Definition op_depends_on_memory (op: operation) : bool :=
   match op with
   | Ocmp (Ccompu _) => negb Archi.ptr64
   | Ocmp (Ccompuimm _ _) => negb Archi.ptr64
-  | Ocmp (Ccomplu _) => Archi.ptr64
-  | Ocmp (Ccompluimm _ _) => Archi.ptr64
   | _ => false
   end.
 
@@ -841,6 +512,7 @@ Qed.
 Definition globals_addressing (addr: addressing) : list ident :=
   match addr with
   | Aglobal s ofs => s :: nil
+  | Abased s ofs => s :: nil
   | _ => nil
   end.
 
@@ -865,13 +537,20 @@ Variable ge2: Genv.t F2 V2.
 Hypothesis agree_on_symbols:
   forall (s: ident), Genv.find_symbol ge2 s = Genv.find_symbol ge1 s.
 
+Remark symbol_address_preserved:
+  forall s ofs, Genv.symbol_address ge2 s ofs = Genv.symbol_address ge1 s ofs.
+Proof.
+  unfold Genv.symbol_address; intros. rewrite agree_on_symbols; auto.
+Qed.
+  
 Lemma eval_addressing_preserved:
   forall sp addr vl,
   eval_addressing ge2 sp addr vl = eval_addressing ge1 sp addr vl.
 Proof.
   intros.
-  unfold eval_addressing; destruct addr; auto. destruct vl; auto. 
-  unfold Genv.symbol_address. rewrite agree_on_symbols; auto.
+  unfold eval_addressing; destruct addr; auto.
+  - destruct vl; auto. rewrite symbol_address_preserved; auto.
+  - unfold Genv.symbol_address. rewrite agree_on_symbols; auto.
 Qed.
 
 Lemma eval_operation_preserved:
@@ -880,7 +559,7 @@ Lemma eval_operation_preserved:
 Proof.
   intros.
   unfold eval_operation; destruct op; auto. destruct vl; auto.
-  unfold Genv.symbol_address. rewrite agree_on_symbols; auto.
+  rewrite symbol_address_preserved; auto.
 Qed.
 
 End GENV_TRANSF.
@@ -951,14 +630,6 @@ Proof.
 - eauto 3 using Val.cmpu_bool_inject, Mem.valid_pointer_implies.
 - inv H3; simpl in H0; inv H0; auto.
 - eauto 3 using Val.cmpu_bool_inject, Mem.valid_pointer_implies.
-- inv H3; inv H2; simpl in H0; inv H0; auto.
-- eauto 3 using Val.cmplu_bool_inject, Mem.valid_pointer_implies.
-- inv H3; simpl in H0; inv H0; auto.
-- eauto 3 using Val.cmplu_bool_inject, Mem.valid_pointer_implies.
-- inv H3; inv H2; simpl in H0; inv H0; auto.
-- inv H3; inv H2; simpl in H0; inv H0; auto.
-- inv H3; inv H2; simpl in H0; inv H0; auto.
-- inv H3; inv H2; simpl in H0; inv H0; auto.
 Qed.
 
 Ltac TrivialExists :=
@@ -996,20 +667,6 @@ Proof.
   - inv H4; inv H2; simpl; auto.
   - inv H4; inv H2; simpl; auto.
   - inv H4; inv H2; simpl; auto.
-  (* div, divu *)
-  - inv H4; inv H3; simpl in H1; inv H1. simpl.
-    destruct (Int.eq i0 Int.zero
-              || Int.eq i (Int.repr Int.min_signed) && Int.eq i0 Int.mone); inv H2.
-    TrivialExists.
-  - inv H4; inv H3; simpl in H1; inv H1. simpl.
-    destruct (Int.eq i0 Int.zero); inv H2. TrivialExists.
-  (* mod, modu *)
-  - inv H4; inv H3; simpl in H1; inv H1. simpl.
-    destruct (Int.eq i0 Int.zero
-                     || Int.eq i (Int.repr Int.min_signed) && Int.eq i0 Int.mone); inv H2.
-    TrivialExists.
-  - inv H4; inv H3; simpl in H1; inv H1. simpl.
-    destruct (Int.eq i0 Int.zero); inv H2. TrivialExists.
   (* and, andimm *)
   - inv H4; inv H2; simpl; auto.
   - inv H4; simpl; auto.
@@ -1031,111 +688,6 @@ Proof.
   (* shrx *)
   - inv H4; simpl in H1; try discriminate. simpl.
     destruct (Int.ltu n (Int.repr 31)); inv H1. TrivialExists.
-  (* makelong, highlong, lowlong *)
-  - inv H4; inv H2; simpl; auto.
-  - inv H4; simpl; auto.
-  - inv H4; simpl; auto.
-  (* cast32 *)
-  - inv H4; simpl; auto.
-  - inv H4; simpl; auto.
-  (* addl, addlimm *)
-  - apply Val.addl_inject; auto.
-  - apply Val.addl_inject; auto.
-  (* negl, subl *)
-  - inv H4; simpl; auto.
-  - apply Val.subl_inject; auto.
-  (* mull, mullhs, mullhu *)
-  - inv H4; inv H2; simpl; auto.
-  - inv H4; inv H2; simpl; auto.
-  - inv H4; inv H2; simpl; auto.
-  (* divl, divlu *)
-  - inv H4; inv H3; simpl in H1; inv H1. simpl.
-    destruct (Int64.eq i0 Int64.zero
-              || Int64.eq i (Int64.repr Int64.min_signed) && Int64.eq i0 Int64.mone); inv H2.
-    TrivialExists.
-  - inv H4; inv H3; simpl in H1; inv H1. simpl.
-    destruct (Int64.eq i0 Int64.zero); inv H2. TrivialExists.
-  (* modl, modlu *)
-  - inv H4; inv H3; simpl in H1; inv H1. simpl.
-    destruct (Int64.eq i0 Int64.zero
-                     || Int64.eq i (Int64.repr Int64.min_signed) && Int64.eq i0 Int64.mone); inv H2.
-    TrivialExists.
-  - inv H4; inv H3; simpl in H1; inv H1. simpl.
-    destruct (Int64.eq i0 Int64.zero); inv H2. TrivialExists.
-  (* andl, andlimm *)
-  - inv H4; inv H2; simpl; auto.
-  - inv H4; simpl; auto.
-  (* orl, orlimm *)
-  - inv H4; inv H2; simpl; auto.
-  - inv H4; simpl; auto.
-  (* xorl, xorlimm *)
-  - inv H4; inv H2; simpl; auto.
-  - inv H4; simpl; auto.
-  (* shll, shllimm *)
-  - inv H4; inv H2; simpl; auto. destruct (Int.ltu i0 Int64.iwordsize'); auto.
-  - inv H4; simpl; auto. destruct (Int.ltu n Int64.iwordsize'); auto.
-  (* shr, shrimm *)
-  - inv H4; inv H2; simpl; auto. destruct (Int.ltu i0 Int64.iwordsize'); auto.
-  - inv H4; simpl; auto. destruct (Int.ltu n Int64.iwordsize'); auto.
-  (* shru, shruimm *)
-  - inv H4; inv H2; simpl; auto. destruct (Int.ltu i0 Int64.iwordsize'); auto.
-  - inv H4; simpl; auto. destruct (Int.ltu n Int64.iwordsize'); auto.
-  (* shrx *)
-  - inv H4; simpl in H1; try discriminate. simpl.
-    destruct (Int.ltu n (Int.repr 63)); inv H1. TrivialExists.
-  (* negf, absf *)
-  - inv H4; simpl; auto.
-  - inv H4; simpl; auto.
-  (* addf, subf *)
-  - inv H4; inv H2; simpl; auto.
-  - inv H4; inv H2; simpl; auto.
-  (* mulf, divf *)
-  - inv H4; inv H2; simpl; auto.
-  - inv H4; inv H2; simpl; auto.
-  (* negfs, absfs *)
-  - inv H4; simpl; auto.
-  - inv H4; simpl; auto.
-  (* addfs, subfs *)
-  - inv H4; inv H2; simpl; auto.
-  - inv H4; inv H2; simpl; auto.
-  (* mulfs, divfs *)
-  - inv H4; inv H2; simpl; auto.
-  - inv H4; inv H2; simpl; auto.
-  (* singleoffloat, floatofsingle *)
-  - inv H4; simpl; auto.
-  - inv H4; simpl; auto.
-  (* intoffloat, intuoffloat *)
-  - inv H4; simpl in H1; inv H1. simpl. destruct (Float.to_int f0); simpl in H2; inv H2.
-    exists (Vint i); auto.
-  - inv H4; simpl in H1; inv H1. simpl. destruct (Float.to_intu f0); simpl in H2; inv H2.
-    exists (Vint i); auto.
-  (* floatofint, floatofintu *)
-  - inv H4; simpl in H1; inv H1. simpl. TrivialExists.
-  - inv H4; simpl in H1; inv H1. simpl. TrivialExists.
-  (* intofsingle, intuofsingle *)
-  - inv H4; simpl in H1; inv H1. simpl. destruct (Float32.to_int f0); simpl in H2; inv H2.
-    exists (Vint i); auto.
-  - inv H4; simpl in H1; inv H1. simpl. destruct (Float32.to_intu f0); simpl in H2; inv H2.
-    exists (Vint i); auto.
-  (* singleofint, singleofintu *)
-  - inv H4; simpl in H1; inv H1. simpl. TrivialExists.
-  - inv H4; simpl in H1; inv H1. simpl. TrivialExists.
-  (* longoffloat, longuoffloat *)
-  - inv H4; simpl in H1; inv H1. simpl. destruct (Float.to_long f0); simpl in H2; inv H2.
-    exists (Vlong i); auto.
-  - inv H4; simpl in H1; inv H1. simpl. destruct (Float.to_longu f0); simpl in H2; inv H2.
-    exists (Vlong i); auto.
-  (* floatoflong, floatoflongu *)
-  - inv H4; simpl in H1; inv H1. simpl. TrivialExists.
-  - inv H4; simpl in H1; inv H1. simpl. TrivialExists.
-  (* longofsingle, longuofsingle *)
-  - inv H4; simpl in H1; inv H1. simpl. destruct (Float32.to_long f0); simpl in H2; inv H2.
-    exists (Vlong i); auto.
-  - inv H4; simpl in H1; inv H1. simpl. destruct (Float32.to_longu f0); simpl in H2; inv H2.
-    exists (Vlong i); auto.
-  (* singleoflong, singleoflongu *)
-  - inv H4; simpl in H1; inv H1. simpl. TrivialExists.
-  - inv H4; simpl in H1; inv H1. simpl. TrivialExists.
   (* cmp *)
   - subst v1. destruct (eval_condition cond vl1 m1) eqn:?.
     exploit eval_condition_inj; eauto. intros EQ; rewrite EQ.
@@ -1153,10 +705,10 @@ Lemma eval_addressing_inj:
   eval_addressing ge1 sp1 addr vl1 = Some v1 ->
   exists v2, eval_addressing ge2 sp2 addr vl2 = Some v2 /\ Val.inject f v1 v2.
 Proof.
-  intros. destruct addr; simpl in H2; simpl; FuncInv; InvInject; TrivialExists.
-  apply Val.offset_ptr_inject; auto.
+  intros. destruct addr; simpl in H2; simpl; FuncInv; InvInject; TrivialExists; auto using Val.add_inject, Val.offset_ptr_inject.
   apply H; simpl; auto.
-  apply Val.offset_ptr_inject; auto. 
+  apply Val.add_inject; auto.
+  apply H; simpl; auto.
 Qed.
 
 End EVAL_COMPAT.
